iris/WpKalloc.v
@@ -26,7 +26,7 @@ Require Import SmodeCore WpSmodeGpr WpMemsetS WpSpinNew WpKernelvecNew WpPushOff
 Require Import WpPushOffMem WpPushOffCsr WpMycpu WpPushOffTop WpMemsetInstr WpHolding WpAcquireMem WpAcquireTop.
 Require Import WpRvcBridge WpLock WpLockLeaves WpHoldingInv WpPopOff.
 Require Import WpAcquireLock WpRelease.
-Require Import KallocInv WpKallocDecode.
+Require Import KallocInv WpKallocDecode WpFreelistMem.
 From Kernel Require KernelInstrs.
 From Kernel Require KernelSyms.
 Local Open Scope Z_scope.
@@ -36,6 +36,8 @@ Section Kalloc.
   Context `{CID : CpuId}.
 
   Notation AK := KernelSyms.kalloc.
+  Notation AQ := KernelSyms.acquire.
+  Notation PO := KernelSyms.push_off.
 
   (* ============================================================= *)
   (* kalloc: whole-function S-mode WP.  WORK IN PROGRESS -- the     *)
@@ -46,6 +48,9 @@ Section Kalloc.
       (γ : gname)
       (m : gmap regidx (mword 64))
       (vr24 vr16 vr8 : bv 64)
+      (svpn_noff svpn_intena svpn_lk svpn_cpu : mword 27)
+      (qvr24 qvr16 qvr8 qpr24 qpr16 qpr8 qpr0 qfraold qfs0old qcpuold : bv 64)
+      (qnoff qintena_old : mword 32) (a0f fl : mword 64)
       (mstatus0 mie_v mdv0 menvcfg0 : mword 64)
       (pmpcfg0 : type_of_register pmpcfg_n) (pmpaddr00 : type_of_register pmpaddr_n)
       (region_pte : PMA_Region) :
@@ -55,6 +60,60 @@ Section Kalloc.
     let a_r16 := add_vec spr (zero_extend' 64 (concat_vec (mword_of_int 2 : mword 6) ('b"000"))) in
     let a_r8  := add_vec spr (zero_extend' 64 (concat_vec (mword_of_int 1 : mword 6) ('b"000"))) in
     let ret_tgt := update_vec_dec (add_vec (m !!! Regidx (mword_of_int 1 : mword 5) : mword 64) (sign_extend' 64 (zeros' 12))) 0 ('b"0") in
+    (* ---- register-map chain through kalloc's prologue + the +0x12 jal ---- *)
+    let R1 := <[Regidx csp_rs1 := regval_into_reg (add_vec (m !!! Regidx csp_rs1) (sign_extend' 64 (sign_extend' 12 (mword_of_int 32 : mword 6))))]> m in
+    let R2 := <[Regidx (mword_of_int 8 : mword 5) := regval_into_reg (add_vec (R1 !!! Regidx csp_rs1) (sign_extend' 64 (caddi4spn_imm (mword_of_int 8 : mword 8))))]> R1 in
+    let R3 := <[Regidx (mword_of_int 10 : mword 5) := regval_into_reg (add_vec (mword_of_int (AK + 0x0a) : mword 64) (auipc_off (mword_of_int 0x11 : mword 20)))]> R2 in
+    let R4 := <[Regidx (mword_of_int 10 : mword 5) := regval_into_reg (add_vec (R3 !!! Regidx (mword_of_int 10 : mword 5)) (sign_extend' 64 (mword_of_int 0x7fe : mword 12)))]> R3 in
+    let mA := <[Regidx (mword_of_int 1 : mword 5) := regval_into_reg (add_vec_int (mword_of_int (AK + 0x12) : mword 64) 4)]> R4 in
+    (* ---- acquire's frame + per-cpu + lock addresses (its [let]s, m := mA) ---- *)
+    let lkA := mA !!! Regidx (mword_of_int 10 : mword 5) in
+    let sp0A := mA !!! Regidx csp_rs1 in
+    let spdA := add_vec sp0A (sign_extend' 64 (sign_extend' 12 (mword_of_int 32 : mword 6))) in
+    let q_r24 := add_vec spdA (zero_extend' 64 (concat_vec (mword_of_int 3 : mword 6) ('b"000"))) in
+    let q_r16 := add_vec spdA (zero_extend' 64 (concat_vec (mword_of_int 2 : mword 6) ('b"000"))) in
+    let q_r8  := add_vec spdA (zero_extend' 64 (concat_vec (mword_of_int 1 : mword 6) ('b"000"))) in
+    let pspdA := add_vec spdA (sign_extend' 64 (sign_extend' 12 (mword_of_int 32 : mword 6))) in
+    let q_p24 := add_vec pspdA (zero_extend' 64 (concat_vec (mword_of_int 3 : mword 6) ('b"000"))) in
+    let q_p16 := add_vec pspdA (zero_extend' 64 (concat_vec (mword_of_int 2 : mword 6) ('b"000"))) in
+    let q_p8  := add_vec pspdA (zero_extend' 64 (concat_vec (mword_of_int 1 : mword 6) ('b"000"))) in
+    let q_p0  := add_vec pspdA (zero_extend' 64 (concat_vec (mword_of_int 0 : mword 6) ('b"000"))) in
+    let pspm10A := add_vec pspdA (sign_extend' 64 (sign_extend' 12 (mword_of_int 48 : mword 6))) in
+    let q_fra := add_vec pspm10A (zero_extend' 64 (concat_vec (mword_of_int 1 : mword 6) ('b"000"))) in
+    let q_fs0 := add_vec pspm10A (zero_extend' 64 (concat_vec (mword_of_int 0 : mword 6) ('b"000"))) in
+    let q_noff := add_vec a0f (sign_extend' 64 (mword_of_int 120 : mword 12)) in
+    let q_intena := add_vec a0f (sign_extend' 64 (mword_of_int 124 : mword 12)) in
+    let q_cpu := add_vec lkA (sign_extend' 64 (mword_of_int 16 : mword 12)) in
+    (* ---- acquire's internal register chain (A0..PN8), m := mA ---- *)
+    let A0 := <[Regidx csp_rs1 := regval_into_reg spdA]> mA in
+    let A1 := <[Regidx (mword_of_int 8 : mword 5) := regval_into_reg
+        (add_vec (A0 !!! Regidx csp_rs1) (sign_extend' 64 (caddi4spn_imm (mword_of_int 8 : mword 8))))]> A0 in
+    let A2 := <[Regidx (mword_of_int 9 : mword 5) := regval_into_reg
+        (add_vec zero_reg (A1 !!! Regidx (mword_of_int 10 : mword 5)))]> A1 in
+    let P0 := <[Regidx (mword_of_int 1 : mword 5) := regval_into_reg
+        (add_vec_int (mword_of_int (AQ + 0x0c) : mword 64) 4)]> A2 in
+    let PN0 := <[Regidx csp_rs1 := regval_into_reg
+        (add_vec (P0 !!! Regidx csp_rs1) (sign_extend' 64 (sign_extend' 12 (mword_of_int 32 : mword 6))))]> P0 in
+    let PN1 := <[Regidx (mword_of_int 8 : mword 5) := regval_into_reg
+        (add_vec (PN0 !!! Regidx csp_rs1) (sign_extend' 64 (caddi4spn_imm (mword_of_int 8 : mword 8))))]> PN0 in
+    let PN2 := <[Regidx (mword_of_int 15 : mword 5) := regval_into_reg (sstatus_read mstatus0)]> PN1 in
+    let PN3 := <[Regidx (mword_of_int 9 : mword 5) := regval_into_reg
+        (add_vec zero_reg (PN2 !!! Regidx (mword_of_int 15 : mword 5)))]> PN2 in
+    let PN4 := po_mycpu_out (mword_of_int (PO + 0x10)) PN3 in
+    let PN5 := <[Regidx (mword_of_int 15 : mword 5) := regval_into_reg (sign_extend' 64 qnoff)]> PN4 in
+    let PN6 := po_mycpu_out (mword_of_int (PO + 0x2c)) PN5 in
+    let PN7 := <[Regidx (mword_of_int 15 : mword 5) := regval_into_reg
+        (shift_bits_right (PN6 !!! Regidx (mword_of_int 9 : mword 5))
+           (subrange_vec_dec (mword_of_int 1 : mword 6) (Z.sub log2_xlen 1) 0))]> PN6 in
+    let PN8 := <[Regidx (mword_of_int 15 : mword 5) := regval_into_reg
+        (and_vec (PN7 !!! Regidx (mword_of_int 15 : mword 5))
+           (sign_extend' 64 (sign_extend' 12 (mword_of_int 1 : mword 6))))]> PN7 in
+    let q_storeval32 := (autocast (T := mword)
+        (subrange_vec_dec (PN8 !!! Regidx (mword_of_int 15 : mword 5)) (Z.sub (Z.mul 4 8) 1) 0) : mword 32) in
+    let q_noff_a5 := sign_extend' 64 (subrange_vec_dec
+        (add_vec (sign_extend' 64 qnoff) (sign_extend' 64 (sign_extend' 12 (mword_of_int 1 : mword 6)))) 31 0) in
+    let q_noff_store := (autocast (T := mword) (subrange_vec_dec q_noff_a5 (Z.sub (Z.mul 4 8) 1) 0) : mword 32) in
+    let q_ret_tgt := update_vec_dec (add_vec (mA !!! Regidx (mword_of_int 1 : mword 5)) (sign_extend' 64 (zeros' 12))) 0 ('b"0") in
     ↑minstretN ⊆ E ->
     ↑lockN ⊆ E ->
     eq_vec (_get_Mstatus_SIE mstatus0) ('b"1") = false ->
@@ -74,6 +133,36 @@ Section Kalloc.
     eq_vec (_get_Pmpcfg_ent_R (vec_access_dec pmpcfg0 0)) ('b"1") = true ->
     (ram_base + ram_size <= uint (vec_access_dec pmpaddr00 0) * 4)%Z ->
     po_mycpu_geom pmpcfg0 pmpaddr00 ->
+    (* ---- acquire's extra side conditions (m := mA) ---- *)
+    legalize_sstatus_val mstatus0 (sstatus_write_val mstatus0 (mword_of_int 2)) = mstatus0 ->
+    (forall pmar0, pma_allows_all pmar0 ->
+       exists region_amo,
+         matching_pma_region pmar0 (Physaddr lkA) 4 = Some region_amo /\
+         (override_PMA (PMA_Region_attributes region_amo) PBMT_PMA).(PMA_readable) = true /\
+         (override_PMA (PMA_Region_attributes region_amo) PBMT_PMA).(PMA_writable) = true /\
+         pma_allows_atomic_op
+           ((override_PMA (PMA_Region_attributes region_amo) PBMT_PMA).(PMA_atomic_support))
+           AMOSWAP 4 = true) ->
+    po_mycpu_out (mword_of_int (PO + 0x10)) PN3 !!! Regidx (mword_of_int 10 : mword 5) = a0f ->
+    po_mycpu_out (mword_of_int (PO + 0x2c)) PN5 !!! Regidx (mword_of_int 10 : mword 5) = a0f ->
+    po_mycpu_out (mword_of_int (PO + 0x18)) PN5 !!! Regidx (mword_of_int 10 : mword 5) = a0f ->
+    po_mycpu_out (mword_of_int (PO + 0x18)) PN8 !!! Regidx (mword_of_int 10 : mword 5) = a0f ->
+    eq_vec (qcpuold : mword 64) (mycpu_ret (mA !!! Regidx (mword_of_int 4 : mword 5))) = false ->
+    po_slot_geom root_ppn pmpaddr00 svpn_noff q_noff 4 ->
+    po_slot_geom root_ppn pmpaddr00 svpn_intena q_intena 4 ->
+    po_slot_geom root_ppn pmpaddr00 svpn_lk lkA 4 ->
+    po_slot_geom root_ppn pmpaddr00 svpn_cpu q_cpu 8 ->
+    eq_vec (access_vec_dec q_ret_tgt 0) ('b"0") = true ->
+    (* the freelist head lives at &kmem.freelist = kmem+24 *)
+    fl = mword_of_int (KernelSyms.kmem + 24) ->
+    (* ---- release's extra side conditions (m := R12) ---- *)
+    eq_vec (_get_MEnvcfg_FIOM menvcfg0) ('b"1") = false ->
+    a0f = mycpu_ret (mA !!! Regidx (mword_of_int 4 : mword 5)) ->
+    neq_vec (and_vec (sstatus_read mstatus0)
+       (sign_extend' 64 (sign_extend' 12 (mword_of_int 2 : mword 6)))) zero_reg = false ->
+    zopz0zKzJ_s zero_reg (sign_extend' 64 q_noff_store) = false ->
+    eq_vec (sign_extend' 64
+       (if eq_vec (sign_extend' 64 qnoff) zero_reg then q_storeval32 else qintena_old)) zero_reg = true ->
     hw_config -∗ minstret_inv -∗
     hart_state ↦ᵣ HART_ACTIVE tt -∗
     cur_privilege ↦ᵣ Supervisor -∗ mstatus ↦ᵣ mstatus0 -∗
@@ -83,6 +172,20 @@ Section Kalloc.
     a_r24 ↦₈ vr24 -∗
     a_r16 ↦₈ vr16 -∗
     a_r8 ↦₈ vr8 -∗
+    (* ---- acquire's scratch-stack windows (below kalloc's own frame) ---- *)
+    q_r24 ↦₈ qvr24 -∗
+    q_r16 ↦₈ qvr16 -∗
+    q_r8  ↦₈ qvr8 -∗
+    q_p24 ↦₈ qpr24 -∗
+    q_p16 ↦₈ qpr16 -∗
+    q_p8  ↦₈ qpr8 -∗
+    q_p0  ↦₈ qpr0 -∗
+    q_fra ↦₈ qfraold -∗
+    q_fs0 ↦₈ qfs0old -∗
+    ([∗ list] j ∈ seq 0 4, (pa_add q_noff j) ↦ₘ nth_byte qnoff j) -∗
+    ([∗ list] j ∈ seq 0 4, (pa_add q_intena j) ↦ₘ nth_byte qintena_old j) -∗
+    is_lock γ lkA (kmem_res fl) -∗
+    q_cpu ↦₈ qcpuold -∗
     ( hart_state ↦ᵣ HART_ACTIVE tt -∗
       cur_privilege ↦ᵣ Supervisor -∗ mstatus ↦ᵣ mstatus0 -∗
       mie ↦ᵣ mie_v -∗ mideleg ↦ᵣ mdv0 -∗ menvcfg ↦ᵣ menvcfg0 -∗
@@ -95,9 +198,16 @@ Section Kalloc.
     WP (Loop : expr riscv_lang) @ E {{ Φ }}.
   Proof.
     intros pcE spr a_r24 a_r16 a_r8 ret_tgt
-      HN HNl HSIE HMPRV HSXL Hmm HMXR Hpmm HPBMTE Hlpe Hpmpp Hpteregion Halignp HW HR Hramcov Hmyg.
+      R1 R2 R3 R4 mA lkA sp0A spdA q_r24 q_r16 q_r8 pspdA q_p24 q_p16 q_p8 q_p0
+      pspm10A q_fra q_fs0 q_noff q_intena q_cpu
+      A0 A1 A2 P0 PN0 PN1 PN2 PN3 PN4 PN5 PN6 PN7 PN8
+      q_storeval32 q_noff_a5 q_noff_store q_ret_tgt
+      HN HNl HSIE HMPRV HSXL Hmm HMXR Hpmm HPBMTE Hlpe Hpmpp Hpteregion Halignp HW HR Hramcov Hmyg
+      Hlegal Hamo Hpin1 Hpin2 Hpin3 Hpin4 Hcpune Hg_noff Hg_int Hg_lk Hg_cpu Hret0 Hfl
+      Hfiom Ha0fcpu Hsst Hnoffpos Hintena0.
     iIntros "#Hhw #Hinv Hhs Hpriv Hms Hmie Hmdl Hmenv Hpmpc Hpmpa Htlbinv
-             #Htext Hpc Hfile Hr24 Hr16 Hr8 Hcont".
+             #Htext Hpc Hfile Hr24 Hr16 Hr8
+             Hqr24 Hqr16 Hqr8 Hqp24 Hqp16 Hqp8 Hqp0 Hqfra Hqfs0 Hnoff Hint #Hlock Hcpu Hcont".
     iPoseProof (kai_00 with "Htext") as "Hi00".
     iPoseProof (kai_02 with "Htext") as "Hi02".
     iPoseProof (kai_04 with "Htext") as "Hi04".
@@ -111,7 +221,6 @@ Section Kalloc.
               HN HSIE HMPRV HSXL Hmm HPBMTE Hmyg Hramcov Hpmpp Hpteregion Halignp ltac:(vm_compute; discriminate)
               with "Hhw Hinv Hhs Hpriv Hms Hmie Hmdl Hmenv Hpmpc Hpmpa Htlbinv Hpc Hfile Hi00 [-]").
     iIntros "Hhs Hpriv Hms Hmie Hmdl Hmenv Hpmpc Hpmpa Htlbinv Hpc Hfile".
-    set (R1 := <[Regidx csp_rs1 := regval_into_reg (add_vec (m !!! Regidx csp_rs1) (sign_extend' 64 (sign_extend' 12 (mword_of_int 32 : mword 6))))]> m).
     assert (HspR1 : R1 !!! Regidx csp_rs1 = spr)
       by (rewrite /R1; apply lookup_total_insert).
     assert (Hpp02 : add_vec_int pcE 2 = mword_of_int (AK + 0x02)) by (apply bv_eq; vm_compute; reflexivity).
@@ -153,7 +262,6 @@ Section Kalloc.
               ltac:(vm_compute; reflexivity) ltac:(vm_compute; discriminate)
               with "Hhw Hinv Hhs Hpriv Hms Hmie Hmdl Hmenv Hpmpc Hpmpa Htlbinv Hpc Hfile Hi08 [-]").
     iIntros "Hhs Hpriv Hms Hmie Hmdl Hmenv Hpmpc Hpmpa Htlbinv Hpc Hfile".
-    set (R2 := <[Regidx (mword_of_int 8 : mword 5) := regval_into_reg (add_vec (R1 !!! Regidx csp_rs1) (sign_extend' 64 (caddi4spn_imm (mword_of_int 8 : mword 8))))]> R1).
     assert (Hpp0a : add_vec_int (mword_of_int (AK + 0x08) : mword 64) 2 = mword_of_int (AK + 0x0a)) by (apply bv_eq; vm_compute; reflexivity).
     iEval (rewrite Hpp0a) in "Hpc".
     (* +0x0a auipc a0,0x11 *)
@@ -162,7 +270,6 @@ Section Kalloc.
               HN HSIE HMPRV HSXL Hmm HPBMTE Hmyg Hramcov Hpmpp Hpteregion Halignp ltac:(vm_compute; discriminate)
               with "Hhw Hinv Hhs Hpriv Hms Hmie Hmdl Hmenv Hpmpc Hpmpa Htlbinv Hpc Hfile Hi0a [-]").
     iIntros "Hhs Hpriv Hms Hmie Hmdl Hmenv Hpmpc Hpmpa Htlbinv Hpc Hfile".
-    set (R3 := <[Regidx (mword_of_int 10 : mword 5) := regval_into_reg (add_vec (mword_of_int (AK + 0x0a) : mword 64) (auipc_off (mword_of_int 0x11 : mword 20)))]> R2).
     assert (Hpp0e : add_vec_int (mword_of_int (AK + 0x0a) : mword 64) 4 = mword_of_int (AK + 0x0e)) by (apply bv_eq; vm_compute; reflexivity).
     iEval (rewrite Hpp0e) in "Hpc".
     (* +0x0e addi a0,a0,2046  (a0 := &kmem) *)
@@ -171,11 +278,267 @@ Section Kalloc.
               HN HSIE HMPRV HSXL Hmm HPBMTE Hmyg Hramcov Hpmpp Hpteregion Halignp ltac:(vm_compute; discriminate)
               with "Hhw Hinv Hhs Hpriv Hms Hmie Hmdl Hmenv Hpmpc Hpmpa Htlbinv Hpc Hfile Hi0e [-]").
     iIntros "Hhs Hpriv Hms Hmie Hmdl Hmenv Hpmpc Hpmpa Htlbinv Hpc Hfile".
-    set (R4 := <[Regidx (mword_of_int 10 : mword 5) := regval_into_reg (add_vec (R3 !!! Regidx (mword_of_int 10 : mword 5)) (sign_extend' 64 (mword_of_int 0x7fe : mword 12)))]> R3).
     assert (Hpp12 : add_vec_int (mword_of_int (AK + 0x0e) : mword 64) 4 = mword_of_int (AK + 0x12)) by (apply bv_eq; vm_compute; reflexivity).
     iEval (rewrite Hpp12) in "Hpc".
-    (* ---- a0 = &kmem now (R4 !!! a0);  +0x12 jal acquire, freelist, release, memset, epilogue TODO ---- *)
-    admit.
+    (* ---- a0 = &kmem now (R4 !!! a0) ---- *)
+    iPoseProof (kai_12 with "Htext") as "Hi12".
+    (* +0x12 jal ra,acquire : link ra := +0x16, jump to acquire's entry *)
+    iDestruct (kv_cfg_split mstatus0 mie_v mdv0 menvcfg0 pmpcfg0 pmpaddr00 HSIE HMPRV HSXL Hmm HPBMTE
+                 with "Hhw Hinv Hhs Hpriv Hms Hmie Hmdl Hmenv Hpmpc Hpmpa")
+      as "(Hsm & Hpca & Hpaa & Hhs2 & Hpriv2 & Hms2 & Hmie2 & Hmdl2 & Hmenv2 & Hpcb & Hpab)".
+    iApply (wp_jal_gpr_s_zca root_ppn E Φ (mword_of_int (AK + 0x12)) (mword_of_int 1 : mword 5) (mword_of_int 0xc8 : mword 21)
+              R4 pmpcfg0 pmpaddr00 region_pte (1/2)%Qp
+              HN Hmyg Hramcov Hpmpp Hpteregion Halignp ltac:(vm_compute; discriminate)
+              ltac:(vm_compute; reflexivity)
+              with "Hhw Hsm Hpca Hpaa Htlbinv Hpc Hfile Hi12 [-]").
+    iIntros "Hsm Hpca Hpaa Htlbinv Hpc Hfile".
+    iDestruct (kv_cfg_recombine mstatus0 mie_v mdv0 menvcfg0 pmpcfg0 pmpaddr00
+                 with "Hsm Hpca Hpaa Hhs2 Hpriv2 Hms2 Hmie2 Hmdl2 Hmenv2 Hpcb Hpab")
+      as "(Hhs & Hpriv & Hms & Hmie & Hmdl & Hmenv & Hpmpc & Hpmpa)".
+    assert (Htgta : add_vec (mword_of_int (AK + 0x12) : mword 64) (sign_extend' 64 (mword_of_int 0xc8 : mword 21)) = mword_of_int KernelSyms.acquire)
+      by (apply bv_eq; vm_compute; reflexivity).
+    iEval (rewrite Htgta) in "Hpc".
+    (* ---- acquire(&kmem): CSL acquire, returns [locked γ ∗ kmem_res fl] ---- *)
+    iApply (wp_acquire_lock root_ppn E Φ γ (kmem_res fl) mA
+              svpn_noff svpn_intena svpn_lk svpn_cpu
+              qvr24 qvr16 qvr8 qpr24 qpr16 qpr8 qfraold qfs0old qcpuold
+              qnoff qintena_old a0f
+              mstatus0 mie_v mdv0 menvcfg0 pmpcfg0 pmpaddr00 region_pte
+              HN HNl HSIE HMPRV HSXL Hmm HMXR Hpmm HPBMTE Hlpe Hpmpp Hpteregion Halignp HW HR Hramcov
+              Hlegal Hamo Hpin1 Hpin2 Hpin3 Hpin4 Hmyg Hcpune Hg_noff Hg_int Hg_lk Hg_cpu Hret0
+              with "Hhw Hinv Hhs Hpriv Hms Hmie Hmdl Hmenv Hpmpc Hpmpa Htlbinv Htext Hpc Hfile
+                    Hqr24 Hqr16 Hqr8 Hqp24 Hqp16 Hqp8 Hqfra Hqfs0 Hnoff Hint Hlock Hcpu [-]").
+    iIntros "Hhs Hpriv Hms Hmie Hmdl Hmenv Hpmpc Hpmpa Htlbinv Hpc Htok HRres Hgpr
+             Hqr24 Hqr16 Hqr8 Hqjunk Hnoff Hint Hcpu".
+    (* ---- acquire returned: [locked γ ∗ kmem_res fl] held, pc = +0x16 ---- *)
+    iDestruct "Hgpr" as (mfin) "[Hfile %Hpins]".
+    destruct Hpins as (Hmra & Hms0 & Hms1 & Hmsp & Hma0 & Hmtp).
+    assert (Hmara : mA !!! Regidx (mword_of_int 1 : mword 5) = add_vec_int (mword_of_int (AK + 0x12) : mword 64) 4)
+      by (rewrite /mA; apply lookup_total_insert).
+    assert (Hpc16 : update_vec_dec (add_vec (mA !!! Regidx (mword_of_int 1 : mword 5)) (sign_extend' 64 (zeros' 12))) 0 ('b"0") = mword_of_int (AK + 0x16)).
+    { rewrite Hmara. apply bv_eq; vm_compute; reflexivity. }
+    iEval (rewrite Hpc16) in "Hpc".
+    iPoseProof (kai_16 with "Htext") as "Hi16".
+    iPoseProof (kai_1a with "Htext") as "Hi1a".
+    iPoseProof (kai_1e with "Htext") as "Hi1e".
+    (* +0x16 auipc s1,0x12 *)
+    iApply (wp_auipc_s root_ppn E Φ (mword_of_int (AK + 0x16)) (mword_of_int 9 : mword 5) (mword_of_int 0x12 : mword 20)
+              mfin mstatus0 mie_v mdv0 menvcfg0 pmpcfg0 pmpaddr00 region_pte (dq:=DfracOwn 1)
+              HN HSIE HMPRV HSXL Hmm HPBMTE Hmyg Hramcov Hpmpp Hpteregion Halignp ltac:(vm_compute; discriminate)
+              with "Hhw Hinv Hhs Hpriv Hms Hmie Hmdl Hmenv Hpmpc Hpmpa Htlbinv Hpc Hfile Hi16 [-]").
+    iIntros "Hhs Hpriv Hms Hmie Hmdl Hmenv Hpmpc Hpmpa Htlbinv Hpc Hfile".
+    set (R6 := <[Regidx (mword_of_int 9 : mword 5) := regval_into_reg (add_vec (mword_of_int (AK + 0x16) : mword 64) (auipc_off (mword_of_int 0x12 : mword 20)))]> mfin).
+    assert (Hs1R6 : R6 !!! Regidx (mword_of_int 9 : mword 5) = add_vec (mword_of_int (AK + 0x16) : mword 64) (auipc_off (mword_of_int 0x12 : mword 20)))
+      by (rewrite /R6; apply lookup_total_insert).
+    assert (Hpp1a : add_vec_int (mword_of_int (AK + 0x16) : mword 64) 4 = mword_of_int (AK + 0x1a)) by (apply bv_eq; vm_compute; reflexivity).
+    iEval (rewrite Hpp1a) in "Hpc".
+    (* +0x1a ld s1,-2038(s1) : s1 := *(kmem.freelist) = head *)
+    iDestruct "HRres" as (head pages) "[Hflw Hchain]".
+    assert (Hldaddr : add_vec (R6 !!! Regidx (mword_of_int 9 : mword 5)) (sign_extend' 64 (mword_of_int 0x80a : mword 12)) = fl).
+    { rewrite Hs1R6 Hfl. apply bv_eq; vm_compute; reflexivity. }
+    iApply (wp_ld_s_ram root_ppn E Φ (mword_of_int (AK + 0x1a)) (mword_of_int 9 : mword 5) (mword_of_int 9 : mword 5) (mword_of_int 0x80a : mword 12)
+              R6 head mstatus0 mie_v mdv0 menvcfg0 pmpcfg0 pmpaddr00 region_pte (dq:=DfracOwn 1) (dqm:=DfracOwn 1)
+              HN ltac:(vm_compute; discriminate) HSIE HMPRV HSXL Hmm HMXR Hpmm HPBMTE Hmyg Hramcov Hpmpp Hpteregion Halignp HR
+              with "Hhw Hinv Hhs Hpriv Hms Hmie Hmdl Hmenv Hpmpc Hpmpa Htlbinv Hpc Hfile Hi1a [Hflw] [-]").
+    { iEval (rewrite -Hldaddr) in "Hflw". rewrite /word_at. iExact "Hflw". }
+    iIntros "Hhs Hpriv Hms Hmie Hmdl Hmenv Hpmpc Hpmpa Htlbinv Hpc Hfile Hflw".
+    iEval (rewrite Hldaddr) in "Hflw".
+    set (R7 := <[Regidx (mword_of_int 9 : mword 5) := regval_into_reg head]> R6).
+    assert (Hs1R7 : R7 !!! Regidx (mword_of_int 9 : mword 5) = head) by (rewrite /R7; apply lookup_total_insert).
+    assert (Hpp1e : add_vec_int (mword_of_int (AK + 0x1a) : mword 64) 4 = mword_of_int (AK + 0x1e)) by (apply bv_eq; vm_compute; reflexivity).
+    iEval (rewrite Hpp1e) in "Hpc".
+    (* +0x1e c.beqz s1,+0x4c : head=nullp -> empty; else pop *)
+    destruct pages as [|p ps].
+    - (* ---- EMPTY list: head = nullp, branch taken to +0x4c ---- *)
+      iDestruct "Hchain" as %Hhead.
+      iApply (wp_cbeqz_taken_s_zca root_ppn E Φ (mword_of_int (AK + 0x1e)) (mword_of_int 23 : mword 8) (Cregidx (mword_of_int 1)) (mword_of_int 9 : mword 5)
+                R7 mstatus0 mie_v mdv0 menvcfg0 pmpcfg0 pmpaddr00 region_pte (dq:=DfracOwn 1)
+                HN HSIE HMPRV HSXL Hmm HPBMTE Hmyg Hramcov Hpmpp Hpteregion Halignp
+                ltac:(vm_compute; reflexivity) ltac:(vm_compute; discriminate)
+                ltac:(rewrite Hs1R7 Hhead; vm_compute; reflexivity)
+                ltac:(vm_compute; reflexivity)
+                with "Hhw Hinv Hhs Hpriv Hms Hmie Hmdl Hmenv Hpmpc Hpmpa Htlbinv Hpc Hfile Hi1e [-]").
+      iIntros "Hhs Hpriv Hms Hmie Hmdl Hmenv Hpmpc Hpmpa Htlbinv Hpc Hfile".
+      (* pc = +0x4c ; empty branch: release, a0:=0, join at +0x40, kalloc_post = nullp *)
+      admit.
+    - (* ---- NONEMPTY: head = p, page_valid p, p <> nullp, fall through to +0x20 ---- *)
+      iDestruct "Hchain" as "(-> & %Hpv & Hrun)".
+      iDestruct "Hrun" as (nxt) "[Hrun Hchain]".
+      iApply (wp_cbeqz_fall_s_config root_ppn E Φ (mword_of_int (AK + 0x1e)) (mword_of_int 23 : mword 8) (Cregidx (mword_of_int 1)) (mword_of_int 9 : mword 5)
+                R7 mstatus0 mie_v mdv0 menvcfg0 pmpcfg0 pmpaddr00 region_pte (dq:=DfracOwn 1)
+                HN HSIE HMPRV HSXL Hmm HPBMTE Hmyg Hramcov Hpmpp Hpteregion Halignp
+                ltac:(vm_compute; reflexivity) ltac:(vm_compute; discriminate)
+                ltac:(rewrite Hs1R7; apply eq_vec_false_iff; intro Hpz;
+                      apply (page_valid_ne_null p Hpv); rewrite Hpz; apply bv_eq; vm_compute; reflexivity)
+                with "Hhw Hinv Hhs Hpriv Hms Hmie Hmdl Hmenv Hpmpc Hpmpa Htlbinv Hpc Hfile Hi1e [-]").
+      iIntros "Hhs Hpriv Hms Hmie Hmdl Hmenv Hpmpc Hpmpa Htlbinv Hpc Hfile".
+      (* pc = +0x20 ; run_page p nxt = word_at p nxt ∗ page_rest p *)
+      iEval (rewrite /run_page) in "Hrun".
+      iDestruct "Hrun" as "[Hpnext Hprest]".
+      iPoseProof (kai_20 with "Htext") as "Hi20".
+      iPoseProof (kai_22 with "Htext") as "Hi22".
+      iPoseProof (kai_26 with "Htext") as "Hi26".
+      (* +0x20 c.ld a5,0(s1) : a5 := *p = nxt *)
+      assert (Hpaddr : add_vec (R7 !!! Regidx (mword_of_int 9 : mword 5))
+                 (sign_extend' 64 (zero_extend' 12 (concat_vec (mword_of_int 0 : mword 5) ('b"000")))) = p).
+      { replace (sign_extend' 64 (zero_extend' 12 (concat_vec (mword_of_int 0 : mword 5) ('b"000"))) : mword 64)
+          with (mword_of_int 0 : mword 64) by (apply bv_eq; vm_compute; reflexivity).
+        rewrite Hs1R7. apply kv_addv_zero. }
+      iApply (wp_cld_s_ram root_ppn E Φ (mword_of_int (AK + 0x20)) (mword_of_int 15 : mword 5) (mword_of_int 9 : mword 5)
+                (zero_extend' 12 (concat_vec (mword_of_int 0 : mword 5) ('b"000")))
+                R7 nxt mstatus0 mie_v mdv0 menvcfg0 pmpcfg0 pmpaddr00 region_pte (dq:=DfracOwn 1) (dqm:=DfracOwn 1)
+                HN ltac:(vm_compute; discriminate) HSIE HMPRV HSXL Hmm HMXR Hpmm HPBMTE Hmyg Hramcov Hpmpp Hpteregion Halignp HR
+                with "Hhw Hinv Hhs Hpriv Hms Hmie Hmdl Hmenv Hpmpc Hpmpa Htlbinv Hpc Hfile Hi20 [Hpnext] [-]").
+      { iEval (rewrite Hpaddr). rewrite /word_at. iExact "Hpnext". }
+      iIntros "Hhs Hpriv Hms Hmie Hmdl Hmenv Hpmpc Hpmpa Htlbinv Hpc Hfile Hpnext".
+      iEval (rewrite Hpaddr) in "Hpnext".
+      set (R8 := <[Regidx (mword_of_int 15 : mword 5) := regval_into_reg nxt]> R7).
+      assert (Hpp22 : add_vec_int (mword_of_int (AK + 0x20) : mword 64) 2 = mword_of_int (AK + 0x22)) by (apply bv_eq; vm_compute; reflexivity).
+      iEval (rewrite Hpp22) in "Hpc".
+      (* +0x22 auipc a4,0x11 *)
+      iApply (wp_auipc_s root_ppn E Φ (mword_of_int (AK + 0x22)) (mword_of_int 14 : mword 5) (mword_of_int 0x11 : mword 20)
+                R8 mstatus0 mie_v mdv0 menvcfg0 pmpcfg0 pmpaddr00 region_pte (dq:=DfracOwn 1)
+                HN HSIE HMPRV HSXL Hmm HPBMTE Hmyg Hramcov Hpmpp Hpteregion Halignp ltac:(vm_compute; discriminate)
+                with "Hhw Hinv Hhs Hpriv Hms Hmie Hmdl Hmenv Hpmpc Hpmpa Htlbinv Hpc Hfile Hi22 [-]").
+      iIntros "Hhs Hpriv Hms Hmie Hmdl Hmenv Hpmpc Hpmpa Htlbinv Hpc Hfile".
+      set (R9 := <[Regidx (mword_of_int 14 : mword 5) := regval_into_reg (add_vec (mword_of_int (AK + 0x22) : mword 64) (auipc_off (mword_of_int 0x11 : mword 20)))]> R8).
+      assert (Ha4R9 : R9 !!! Regidx (mword_of_int 14 : mword 5) = add_vec (mword_of_int (AK + 0x22) : mword 64) (auipc_off (mword_of_int 0x11 : mword 20)))
+        by (rewrite /R9; apply lookup_total_insert).
+      assert (Ha5R9 : R9 !!! Regidx (mword_of_int 15 : mword 5) = nxt).
+      { rewrite /R9 lookup_total_insert_ne; [| vm_compute; discriminate]. rewrite /R8; apply lookup_total_insert. }
+      assert (Hpp26 : add_vec_int (mword_of_int (AK + 0x22) : mword 64) 4 = mword_of_int (AK + 0x26)) by (apply bv_eq; vm_compute; reflexivity).
+      iEval (rewrite Hpp26) in "Hpc".
+      (* +0x26 sd a5,2046(a4) : kmem.freelist := nxt *)
+      assert (Hstaddr : add_vec (R9 !!! Regidx (mword_of_int 14 : mword 5)) (sign_extend' 64 (mword_of_int 0x7fe : mword 12)) = fl).
+      { rewrite Ha4R9 Hfl. apply bv_eq; vm_compute; reflexivity. }
+      iApply (wp_sd_s_ram root_ppn E Φ (mword_of_int (AK + 0x26)) (mword_of_int 15 : mword 5) (mword_of_int 14 : mword 5) (mword_of_int 0x7fe : mword 12)
+                R9 p mstatus0 mie_v mdv0 menvcfg0 pmpcfg0 pmpaddr00 region_pte (dq:=DfracOwn 1)
+                HN HSIE HMPRV HSXL Hmm HMXR Hpmm HPBMTE Hmyg Hramcov Hpmpp Hpteregion Halignp HW
+                with "Hhw Hinv Hhs Hpriv Hms Hmie Hmdl Hmenv Hpmpc Hpmpa Htlbinv Hpc Hfile Hi26 [Hflw] [-]").
+      { iEval (rewrite -Hstaddr) in "Hflw". rewrite /word_at. iExact "Hflw". }
+      iIntros "Hhs Hpriv Hms Hmie Hmdl Hmenv Hpmpc Hpmpa Htlbinv Hpc Hfile Hflw".
+      rewrite Ha5R9. iEval (rewrite Hstaddr) in "Hflw".
+      (* reclose kmem_res fl on the new head nxt, and reassemble page_own p *)
+      iAssert (kmem_res fl) with "[Hflw Hchain]" as "HRres".
+      { iApply (kmem_res_close fl nxt ps). rewrite /word_at. iFrame "Hflw Hchain". }
+      iAssert (page_own p) with "[Hpnext Hprest]" as "Hpage".
+      { iApply (run_page_page_own p nxt). rewrite /run_page /word_at. iFrame "Hpnext Hprest". }
+      assert (Hpp2a : add_vec_int (mword_of_int (AK + 0x26) : mword 64) 4 = mword_of_int (AK + 0x2a)) by (apply bv_eq; vm_compute; reflexivity).
+      iEval (rewrite Hpp2a) in "Hpc".
+      iPoseProof (kai_2a with "Htext") as "Hi2a".
+      iPoseProof (kai_2e with "Htext") as "Hi2e".
+      (* +0x2a auipc a0,0x11 *)
+      iApply (wp_auipc_s root_ppn E Φ (mword_of_int (AK + 0x2a)) (mword_of_int 10 : mword 5) (mword_of_int 0x11 : mword 20)
+                R9 mstatus0 mie_v mdv0 menvcfg0 pmpcfg0 pmpaddr00 region_pte (dq:=DfracOwn 1)
+                HN HSIE HMPRV HSXL Hmm HPBMTE Hmyg Hramcov Hpmpp Hpteregion Halignp ltac:(vm_compute; discriminate)
+                with "Hhw Hinv Hhs Hpriv Hms Hmie Hmdl Hmenv Hpmpc Hpmpa Htlbinv Hpc Hfile Hi2a [-]").
+      iIntros "Hhs Hpriv Hms Hmie Hmdl Hmenv Hpmpc Hpmpa Htlbinv Hpc Hfile".
+      set (R10 := <[Regidx (mword_of_int 10 : mword 5) := regval_into_reg (add_vec (mword_of_int (AK + 0x2a) : mword 64) (auipc_off (mword_of_int 0x11 : mword 20)))]> R9).
+      assert (Hpp2e : add_vec_int (mword_of_int (AK + 0x2a) : mword 64) 4 = mword_of_int (AK + 0x2e)) by (apply bv_eq; vm_compute; reflexivity).
+      iEval (rewrite Hpp2e) in "Hpc".
+      (* +0x2e addi a0,a0,2014  (a0 := &kmem) *)
+      iApply (wp_addi4_s root_ppn E Φ (mword_of_int (AK + 0x2e)) (mword_of_int 10 : mword 5) (mword_of_int 10 : mword 5) (mword_of_int 0x7de : mword 12)
+                R10 mstatus0 mie_v mdv0 menvcfg0 pmpcfg0 pmpaddr00 region_pte (dq:=DfracOwn 1)
+                HN HSIE HMPRV HSXL Hmm HPBMTE Hmyg Hramcov Hpmpp Hpteregion Halignp ltac:(vm_compute; discriminate)
+                with "Hhw Hinv Hhs Hpriv Hms Hmie Hmdl Hmenv Hpmpc Hpmpa Htlbinv Hpc Hfile Hi2e [-]").
+      iIntros "Hhs Hpriv Hms Hmie Hmdl Hmenv Hpmpc Hpmpa Htlbinv Hpc Hfile".
+      set (R11 := <[Regidx (mword_of_int 10 : mword 5) := regval_into_reg (add_vec (R10 !!! Regidx (mword_of_int 10 : mword 5)) (sign_extend' 64 (mword_of_int 0x7de : mword 12)))]> R10).
+      assert (Ha0kmem : R11 !!! Regidx (mword_of_int 10 : mword 5) = mword_of_int KernelSyms.kmem).
+      { rewrite /R11 lookup_total_insert /R10 lookup_total_insert. apply bv_eq; vm_compute; reflexivity. }
+      assert (Hpp32 : add_vec_int (mword_of_int (AK + 0x2e) : mword 64) 4 = mword_of_int (AK + 0x32)) by (apply bv_eq; vm_compute; reflexivity).
+      iEval (rewrite Hpp32) in "Hpc".
+      iPoseProof (kai_32 with "Htext") as "Hi32".
+      (* +0x32 jal ra,release : link ra := +0x36, jump to release's entry *)
+      iDestruct (kv_cfg_split mstatus0 mie_v mdv0 menvcfg0 pmpcfg0 pmpaddr00 HSIE HMPRV HSXL Hmm HPBMTE
+                   with "Hhw Hinv Hhs Hpriv Hms Hmie Hmdl Hmenv Hpmpc Hpmpa")
+        as "(Hsm & Hpca & Hpaa & Hhs2 & Hpriv2 & Hms2 & Hmie2 & Hmdl2 & Hmenv2 & Hpcb & Hpab)".
+      iApply (wp_jal_gpr_s_zca root_ppn E Φ (mword_of_int (AK + 0x32)) (mword_of_int 1 : mword 5) (mword_of_int 0x130 : mword 21)
+                R11 pmpcfg0 pmpaddr00 region_pte (1/2)%Qp
+                HN Hmyg Hramcov Hpmpp Hpteregion Halignp ltac:(vm_compute; discriminate)
+                ltac:(vm_compute; reflexivity)
+                with "Hhw Hsm Hpca Hpaa Htlbinv Hpc Hfile Hi32 [-]").
+      iIntros "Hsm Hpca Hpaa Htlbinv Hpc Hfile".
+      iDestruct (kv_cfg_recombine mstatus0 mie_v mdv0 menvcfg0 pmpcfg0 pmpaddr00
+                   with "Hsm Hpca Hpaa Hhs2 Hpriv2 Hms2 Hmie2 Hmdl2 Hmenv2 Hpcb Hpab")
+        as "(Hhs & Hpriv & Hms & Hmie & Hmdl & Hmenv & Hpmpc & Hpmpa)".
+      set (R12 := <[Regidx (mword_of_int 1 : mword 5) := regval_into_reg (add_vec_int (mword_of_int (AK + 0x32) : mword 64) 4)]> R11).
+      assert (Htgtr : add_vec (mword_of_int (AK + 0x32) : mword 64) (sign_extend' 64 (mword_of_int 0x130 : mword 21)) = mword_of_int KernelSyms.release)
+        by (apply bv_eq; vm_compute; reflexivity).
+      iEval (rewrite Htgtr) in "Hpc".
+      (* pc = release entry, a0 = &kmem, ra = +0x36 ; hold locked γ ∗ kmem_res fl. *)
+      (* ---- register-agreement facts across the R6..R12 chain (m := R12) ---- *)
+      assert (HR12csp : R12 !!! Regidx csp_rs1 = mA !!! Regidx csp_rs1).
+      { rewrite /R12 lookup_total_insert_ne; [| vm_compute; discriminate].
+        rewrite /R11 lookup_total_insert_ne; [| vm_compute; discriminate].
+        rewrite /R10 lookup_total_insert_ne; [| vm_compute; discriminate].
+        rewrite /R9 lookup_total_insert_ne; [| vm_compute; discriminate].
+        rewrite /R8 lookup_total_insert_ne; [| vm_compute; discriminate].
+        rewrite /R7 lookup_total_insert_ne; [| vm_compute; discriminate].
+        rewrite /R6 lookup_total_insert_ne; [| vm_compute; discriminate].
+        exact Hmsp. }
+      assert (HR12tp : R12 !!! Regidx (mword_of_int 4 : mword 5) = mA !!! Regidx (mword_of_int 4 : mword 5)).
+      { rewrite /R12 lookup_total_insert_ne; [| vm_compute; discriminate].
+        rewrite /R11 lookup_total_insert_ne; [| vm_compute; discriminate].
+        rewrite /R10 lookup_total_insert_ne; [| vm_compute; discriminate].
+        rewrite /R9 lookup_total_insert_ne; [| vm_compute; discriminate].
+        rewrite /R8 lookup_total_insert_ne; [| vm_compute; discriminate].
+        rewrite /R7 lookup_total_insert_ne; [| vm_compute; discriminate].
+        rewrite /R6 lookup_total_insert_ne; [| vm_compute; discriminate].
+        exact Hmtp. }
+      assert (HR12a0 : R12 !!! Regidx (mword_of_int 10 : mword 5) = mword_of_int KernelSyms.kmem).
+      { rewrite /R12 lookup_total_insert_ne; [| vm_compute; discriminate]. exact Ha0kmem. }
+      assert (HR12ra : R12 !!! Regidx (mword_of_int 1 : mword 5) = add_vec_int (mword_of_int (AK + 0x32) : mword 64) 4)
+        by (rewrite /R12; apply lookup_total_insert).
+      assert (HlkAkmem : lkA = mword_of_int KernelSyms.kmem).
+      { rewrite /lkA /mA lookup_total_insert_ne; [| vm_compute; discriminate].
+        rewrite /R4 lookup_total_insert /R3 lookup_total_insert.
+        apply bv_eq; vm_compute; reflexivity. }
+      (* ---- release's window addresses reduce to kalloc's q_* slots ---- *)
+      assert (Hacpu : add_vec (R12 !!! Regidx (mword_of_int 10 : mword 5)) (sign_extend' 64 (mword_of_int 16 : mword 12)) = q_cpu).
+      { rewrite HR12a0 /q_cpu HlkAkmem. reflexivity. }
+      assert (Hanoff : add_vec (mycpu_ret (R12 !!! Regidx (mword_of_int 4 : mword 5))) (sign_extend' 64 (mword_of_int 120 : mword 12)) = q_noff).
+      { rewrite HR12tp /q_noff Ha0fcpu. reflexivity. }
+      assert (Haint : add_vec (mycpu_ret (R12 !!! Regidx (mword_of_int 4 : mword 5))) (sign_extend' 64 (mword_of_int 124 : mword 12)) = q_intena).
+      { rewrite HR12tp /q_intena Ha0fcpu. reflexivity. }
+      iDestruct "Hqjunk" as (vp24 vp16 vp8 vfra vfs0) "(Hqp24 & Hqp16 & Hqp8 & Hqfra & Hqfs0)".
+      iApply (wp_release root_ppn E Φ γ lkA (kmem_res fl) R12
+                svpn_lk svpn_cpu svpn_noff svpn_intena
+                (mycpu_ret (mA !!! Regidx (mword_of_int 4 : mword 5)))
+                q_noff_store
+                (if eq_vec (sign_extend' 64 qnoff) zero_reg then q_storeval32 else qintena_old)
+                (mA !!! Regidx (mword_of_int 1 : mword 5))
+                (mA !!! Regidx (mword_of_int 8 : mword 5))
+                (mA !!! Regidx (mword_of_int 9 : mword 5))
+                vp24 vp16 vp8 qpr0 vfra vfs0
+                mstatus0 mie_v mdv0 menvcfg0 pmpcfg0 pmpaddr00 region_pte (dqi:=DfracOwn 1)
+                HN HNl HSIE HMPRV HSXL Hmm HMXR Hpmm HPBMTE Hfiom Hlpe Hpmpp Hpteregion Halignp HW HR Hramcov Hmyg
+                ltac:(rewrite HR12a0 HlkAkmem; apply bv_eq; vm_compute; reflexivity)
+                Hg_lk
+                ltac:(rewrite Hacpu; exact Hg_cpu)
+                ltac:(rewrite Hanoff; exact Hg_noff)
+                ltac:(rewrite Haint; exact Hg_int)
+                ltac:(rewrite HR12tp; apply eq_vec_true_iff; reflexivity)
+                Hsst Hnoffpos Hintena0
+                ltac:(rewrite HR12ra; vm_compute; reflexivity)
+                with "Hhw Hinv Hhs Hpriv Hms Hmie Hmdl Hmenv Hpmpc Hpmpa Htlbinv Htext Hpc Hfile
+                      Hlock Htok HRres [Hcpu] [Hnoff] [Hint] [Hqr24] [Hqr16] [Hqr8]
+                      [Hqp24] [Hqp16] [Hqp8] [Hqp0] [Hqfra] [Hqfs0] [-]").
+      { iEval (rewrite Hacpu). iExact "Hcpu". }
+      { iEval (rewrite Hanoff). iExact "Hnoff". }
+      { iEval (rewrite Haint). iExact "Hint". }
+      { iEval (rewrite HR12csp). iExact "Hqr24". }
+      { iEval (rewrite HR12csp). iExact "Hqr16". }
+      { iEval (rewrite HR12csp). iExact "Hqr8". }
+      { iEval (rewrite HR12csp). iExact "Hqp24". }
+      { iEval (rewrite HR12csp). iExact "Hqp16". }
+      { iEval (rewrite HR12csp). iExact "Hqp8". }
+      { iEval (rewrite HR12csp). iExact "Hqp0". }
+      { iEval (rewrite HR12csp). iExact "Hqfra". }
+      { iEval (rewrite HR12csp). iExact "Hqfs0". }
+      iIntros "Hhs Hpriv Hms Hmie Hmdl Hmenv Hpmpc Hpmpa Htlbinv Hpc Hgpr2 Hcpu2 Hnoff2 Hint2 Hjunk2".
+      (* pc = ret_tgt = +0x36 ; lock released, still hold [page_own p].
+         memset(p, 0, 4096); a0 := p; epilogue.  TODO *)
+      admit.
   Admitted.
 
 End Kalloc.
